examples/dm4free/FStar.DM4F.IntStoreExcFixed.fst
@@ -27,8 +27,8 @@ let bind_is (a b : Type) (x:int_store_exc a) (f: a -> int_store_exc b) : int_sto
     | None -> None, store'
     | Some xa -> f xa store'
 
-let get () : int_store_exc (heap) = fun store -> Some store, store
-let put s : int_store_exc unit = fun _ -> Some (), s
+let iget () : int_store_exc (heap) = fun store -> Some store, store
+let iput s : int_store_exc unit = fun _ -> Some (), s
 
 (* DM4F does not handle polymorphic types yet so we go around this limitation *)
 (* by returning an inhabitant of False and define a second polymorphic raise_ afterwards *)
@@ -39,10 +39,13 @@ total reifiable reflectable new_effect {
   with repr   = int_store_exc
      ; bind   = bind_is
      ; return = return_is
-     ; get   = get
-     ; put    = put
+     ; get   = iget
+     ; put    = iput
      ; raise_ = raise_impl
 }
+
+let get = INT_STORE_EXC?.get
+let put = INT_STORE_EXC?.put
 
 effect IntStoreExc (a:Type) (pre:INT_STORE_EXC?.pre) (post: heap -> option a -> heap -> GTot Type0) =
   INT_STORE_EXC a (fun l0 p -> pre l0 /\ (forall x l1. pre l0 /\ post l0 x l1 ==> p (x, l1)))
